define flattening for expressions and statements, and prove it correct for expressions, modulo some "unmodified vars" conditions

src/Common.v
@@ -1,12 +1,17 @@
+Require Export Coq.omega.Omega.
+Require Export bbv.Word.
 Require Export compiler.Monad.
 Require Export compiler.Decidable.
-Require Export bbv.Word.
+Require Export compiler.Tactics.
 
 Class Map(T K V: Type) := mMap {
   empty: T;
   get: T -> K -> option V;
   put: T -> K -> V -> T;
-  (* TODO probably needs some properties *)
+
+  get_put_same: forall (m: T) (k: K) (v: V), get (put m k v) k = Some v;
+  get_put_diff: forall (m: T) (k1 k2: K) (v: V), k1 <> k2 -> get (put m k1 v) k2 = get m k2
+  (* TODO probably needs some more properties *)
 }.
 
 Instance Function_Map(K V: Type){decK: DecidableEq K}: Map (K -> option V) K V := {|
@@ -15,5 +20,12 @@ Instance Function_Map(K V: Type){decK: DecidableEq K}: Map (K -> option V) K V :
   put := fun (m: K -> option V) (k: K) (v: V) =>
            fun (k': K) => if dec (k = k') then Some v else m k'
 |}.
+- intros. cbv. destruct_one_match; reflexivity || contradiction.
+- intros. cbv. destruct_one_match; reflexivity || contradiction.
+Defined.
 
 Global Instance dec_eq_word : forall sz, DecidableEq (word sz) := weq.
+
+(* We want assign ranges of variables for certain purposes, so we need a total order,
+   and we want S for to generate a fresh variable, so let's just use nat. *)
+Definition var := nat.
