src/FlattenExpr.v
@@ -1,0 +1,434 @@
+Require Import lib.LibTactics.
+Require Import compiler.Common.
+Require Import compiler.ResMonad.
+Require compiler.ExprImp.
+Require compiler.FlatImp.
+
+
+Section FlattenExpr.
+
+  Context {w: nat}. (* bit width *)
+  Context {state: Type}.
+  Context {stateMap: Map state var (word w)}.
+
+  (* returns statement and var into which result is saved, and that's the highest used var *)
+  Fixpoint flattenExpr(firstFree: var)(e: @ExprImp.expr w): (@FlatImp.stmt w * var) :=
+    match e with
+    | ExprImp.ELit n => (FlatImp.SLit firstFree n, firstFree)
+    | ExprImp.EVar x => (FlatImp.SSet firstFree x, firstFree)
+       (* returning "(FlatImp.SSkip, x)" would be simpler but that doesn't respect the invariant
+          that the returned var is >= firstFree *)
+    | ExprImp.EOp op e1 e2 =>
+        let (p1, r1) := flattenExpr firstFree e1 in
+        let (p2, r2) := flattenExpr (S r1) e2 in
+        (FlatImp.SSeq p1 (FlatImp.SSeq p2 (FlatImp.SOp (S r2) op r1 r2)), S r2)
+    end.
+
+  (* returns statement and new first free var *)
+  Fixpoint flattenStmt(firstFree: var)(s: @ExprImp.stmt w): (@FlatImp.stmt w * var) :=
+    match s with
+    | ExprImp.SSet x e =>
+        let (e', r) := flattenExpr firstFree e in
+        (FlatImp.SSeq e' (FlatImp.SSet x r), S r)
+    | ExprImp.SIf cond sThen sElse =>
+        let (cond', r1) := flattenExpr firstFree cond in
+        let (sThen', f2) := flattenStmt (S r1) sThen in
+        let (sElse', f3) := flattenStmt f2 sElse in
+        (FlatImp.SSeq cond' (FlatImp.SIf r1 sThen' sElse'), f3)
+    | ExprImp.SWhile cond body =>
+        let (cond', r1) := flattenExpr firstFree cond in
+        let (body', f2) := flattenStmt (S r1) body in
+        (FlatImp.SLoop cond' r1 body', f2)
+    | ExprImp.SSeq s1 s2 =>
+        let (s1', f1) := flattenStmt firstFree s1 in
+        let (s2', f2) := flattenStmt f1 s2 in
+        (FlatImp.SSeq s1' s2', f2)
+    | ExprImp.SSkip => (FlatImp.SSkip, firstFree)
+    end.
+
+  (* Alternative:
+
+  (* returns statement, var into which result is saved, and new first free var *)
+  Fixpoint flattenExpr(firstFree: var)(e: @ExprImp.expr w): (@FlatImp.stmt w * var * var) :=
+    match e with
+    | ExprImp.ELit n => (FlatImp.SLit firstFree n, firstFree, S firstFree)
+    | ExprImp.EVar x => (FlatImp.SSkip, x, firstFree)
+    | ExprImp.EOp op e1 e2 =>
+        let '(p1, r1, f1) := flattenExpr firstFree e1 in
+        let '(p2, r2, f2) := flattenExpr f1 e2 in
+        (FlatImp.SSeq p1 (FlatImp.SSeq p2 (FlatImp.SOp (S f2) op r1 r2)), S f2, S (S f2))
+    end.
+  *)
+
+  (* Alternative (violates "extends finalL initialL"):
+
+  (* returns statement and new first free var *)
+  Fixpoint flattenExpr(firstFree res: var)(e: @ExprImp.expr w): (@FlatImp.stmt w * var) :=
+    match e with
+    | ExprImp.ELit n => (FlatImp.SLit res n, firstFree)
+    | ExprImp.EVar x => (FlatImp.SSet res x, firstFree)
+    | ExprImp.EOp op e1 e2 =>
+        let (p1, f1) := flattenExpr (S firstFree) firstFree e1 in
+        let (p2, f2) := flattenExpr (S f1) f1 e2 in
+        (FlatImp.SSeq p1 (FlatImp.SSeq p2 (FlatImp.SOp res op firstFree f1)), f2)
+    end.
+
+  (* returns statement and new first free var *)
+  Fixpoint flattenStmt(firstFree: var)(s: @ExprImp.stmt w): (@FlatImp.stmt w * var) :=
+    match s with
+    | ExprImp.SSet x e => flattenExpr firstFree x e
+    | ExprImp.SIf cond sThen sElse =>
+        let (cond', f1) := flattenExpr (S firstFree) firstFree cond in
+        let (sThen', f2) := flattenStmt f1 sThen in
+        let (sElse', f3) := flattenStmt f2 sElse in
+        (FlatImp.SSeq cond' (FlatImp.SIf firstFree sThen' sElse'), f3)
+    | ExprImp.SWhile cond body =>
+        let (cond', f1) := flattenExpr (S firstFree) firstFree cond in
+        let (body', f2) := flattenStmt f1 body in
+        (FlatImp.SLoop cond' firstFree body', f2)
+    | ExprImp.SSeq s1 s2 =>
+        let (s1', f1) := flattenStmt firstFree s1 in
+        let (s2', f2) := flattenStmt f1 s2 in
+        (FlatImp.SSeq s1' s2', f2)
+    | ExprImp.SSkip => (FlatImp.SSkip, firstFree)
+    end.
+  *)
+
+  Definition extends(s1 s2: state) := forall x v, get s2 x = Some v -> get s1 x = Some v.
+
+  Lemma put_extends: forall s x v,
+    extends (put s x v) s.
+  Proof. unfold extends. intros. Abort.
+
+  Definition var_range := (var * var)%type.
+
+  Definition range_empty: var_range := (0, 0).
+
+  Definition range_one(x: var): var_range := (x, S x).
+
+  Definition range_add(new lo hi: var): var_range :=
+    if dec (lo = hi) then (new, new) else (min new lo, max new hi).
+
+  Definition range_union(r1 r2: var_range): var_range :=
+    let (lo1, hi1) := r1 in let (lo2, hi2) := r2 in
+    if dec (lo1 = hi1) then r2 else if dec (lo2 = hi2) then r1 else (min lo1 lo2, max hi1 hi2).
+
+  (* returns the set of modified vars (always a contiguous range, end points to first unmodified) *)
+  Fixpoint modVars(s: @FlatImp.stmt w): var_range :=
+    match s with
+    | FlatImp.SLit x v => range_one x
+    | FlatImp.SOp x op y z => range_one x
+    | FlatImp.SSet x y => range_one x
+    | FlatImp.SIf cond bThen bElse =>
+        range_union (modVars bThen) (modVars bElse)
+    | FlatImp.SLoop body1 cond body2 =>
+        range_union (modVars body1) (modVars body2)
+    | FlatImp.SSeq s1 s2 =>
+        range_union (modVars s1) (modVars s2)
+    | FlatImp.SSkip => range_empty
+    end.
+
+  Definition only_differ(s1: state)(r: var_range)(s2: state) :=
+    forall x, x < fst r \/ x >= snd r -> get s1 x = get s2 x.
+
+Ltac destruct_one_match_hyp_test type_test :=
+  match goal with
+  | H: context[match ?e with _ => _ end] |- _ =>
+      is_var e;
+      let T := type of e in type_test T;
+      destruct e
+  | H: context[if ?e then _ else _] |- _ =>
+      is_var e;
+      let T := type of e in type_test T;
+      destruct e
+  | H: context[match ?e with _ => _ end] |- _ =>
+      let T := type of e in type_test T;
+      let E := fresh "E" in destruct e eqn: E
+  | H: context[if ?e then _ else _] |- _ =>
+      let T := type of e in type_test T;
+      let E := fresh "E" in destruct e eqn: E
+  end.
+
+Ltac destruct_one_match_hyp_of_type T :=
+  destruct_one_match_hyp_test ltac:(fun t => unify t T).
+
+Ltac destruct_one_match_hyp :=
+  destruct_one_match_hyp_test ltac:(fun t => idtac).
+
+Ltac inversionss :=
+  repeat match goal with
+  | H: ?a = ?b |- _ => inversion H; subst; clear H;
+                       match goal with
+                       | H': a = b |- _ => fail 1
+                       | _ => idtac
+                       end
+  end.
+
+  Definition valid_range(r: var_range) := fst r <= snd r.
+
+  Lemma only_differ_union_l: forall s1 s2 r1 r2,
+    valid_range r1 ->
+    valid_range r2 ->
+    only_differ s1 r1 s2 ->
+    only_differ s1 (range_union r1 r2) s2.
+  Proof.
+    cbv [only_differ range_union]. introv R1 R2 D B. destruct r1 as [lo1 hi1], r2 as [lo2 hi2].
+    pose proof (Min.min_spec lo1 lo2).
+    pose proof (Max.max_spec hi1 hi2).
+    repeat destruct_one_match_hyp; subst; simpl in *; apply D; omega.
+  Qed.
+
+  Lemma only_differ_union_r: forall s1 s2 r1 r2,
+    valid_range r1 ->
+    valid_range r2 ->
+    only_differ s1 r2 s2 ->
+    only_differ s1 (range_union r1 r2) s2.
+  Proof.
+    cbv [only_differ range_union]. introv R1 R2 D B. destruct r1 as [lo1 hi1], r2 as [lo2 hi2].
+    pose proof (Min.min_spec lo1 lo2).
+    pose proof (Max.max_spec hi1 hi2).
+    repeat destruct_one_match_hyp; subst; simpl in *; apply D; omega.
+  Qed.
+
+  Lemma union_preserves_valid_range: forall r1 r2,
+    valid_range r1 ->
+    valid_range r2 ->
+    valid_range (range_union r1 r2).
+  Proof.
+    intros. destruct r1 as [lo1 hi1], r2 as [lo2 hi2].
+    pose proof (Min.min_spec lo1 lo2).
+    pose proof (Max.max_spec hi1 hi2).
+    unfold valid_range, range_union in *.
+    repeat destruct_one_match; subst; simpl in *; omega.
+  Qed.
+
+  Lemma valid_range_modVars: forall s,
+    valid_range (modVars s).
+  Proof.
+    induction s;
+    unfold valid_range, modVars; simpl; try omega; fold modVars;
+    apply union_preserves_valid_range; assumption.
+  Qed.
+
+  Lemma only_differ_one: forall s x v,
+    only_differ s (range_one x) (put s x v).
+  Proof.
+    unfold only_differ, range_one. intros. symmetry. apply get_put_diff. simpl in *. omega.
+  Qed.
+
+  Lemma only_differ_refl: forall s1 r,
+    only_differ s1 r s1.
+  Proof.
+    unfold only_differ. intros. reflexivity.
+  Qed.
+
+  Lemma only_differ_sym: forall s1 s2 r,
+    only_differ s1 r s2 ->
+    only_differ s2 r s1.
+  Proof.
+    unfold only_differ. intros. symmetry. auto.
+  Qed.
+
+  Lemma only_differ_trans: forall s1 s2 s3 r,
+    only_differ s1 r s2 ->
+    only_differ s2 r s3 ->
+    only_differ s1 r s3.
+  Proof.
+    unfold only_differ. introv E1 E2 B. destruct r as [lo hi]. simpl in *.
+    rewrite E1 by omega. rewrite E2 by omega. reflexivity.
+  Qed.
+
+  Lemma invert_eval_SLoop: forall fuel st1 body1 cond body2 st4,
+    FlatImp.eval_stmt (S fuel) st1 (FlatImp.SLoop body1 cond body2) = Success st4 ->
+    FlatImp.eval_stmt fuel st1 body1 = Success st4 /\ get st4 cond = Some $0 \/
+    exists st2 st3 cv, FlatImp.eval_stmt fuel st1 body1 = Success st2 /\
+                       get st2 cond = Some cv /\ cv <> $0 /\
+                       FlatImp.eval_stmt fuel st2 body2 = Success st3 /\
+                       FlatImp.eval_stmt fuel st3 (FlatImp.SLoop body1 cond body2) = Success st4.
+  Proof.
+    introv Ev. simpl in Ev. unfold option2res in *.
+    repeat (destruct_one_match_hyp; try discriminate); inversionss; eauto 10.
+  Qed.
+
+  Lemma invert_eval_SSeq: forall fuel initial s1 s2 final,
+    FlatImp.eval_stmt (S fuel) initial (FlatImp.SSeq s1 s2) = Success final ->
+    exists mid, FlatImp.eval_stmt fuel initial s1 = Success mid /\
+                FlatImp.eval_stmt fuel mid s2 = Success final.
+  Proof.
+    introv Ev. simpl in Ev. destruct_one_match_hyp; try discriminate. eauto.
+  Qed.
+
+  Lemma modVarsSound: forall fuel s initial final,
+    FlatImp.eval_stmt fuel initial s = Success final ->
+    only_differ initial (modVars s) final.
+  Proof.
+    induction fuel; introv Ev.
+    - discriminate.
+    - destruct s.
+      + simpl in *. inversionss. apply only_differ_one.
+      + simpl in Ev. unfold option2res in *.
+        repeat (destruct_one_match_hyp_of_type (option (word w)); try discriminate).
+        inversionss. apply only_differ_one.
+      + simpl in Ev. unfold option2res in *.
+        repeat (destruct_one_match_hyp_of_type (option (word w)); try discriminate).
+        inversionss. apply only_differ_one.
+      + simpl in *. unfold option2res in *.
+        repeat (destruct_one_match_hyp_of_type (option (word w)); try discriminate).
+        destruct fuel; [ inversion Ev | ].
+        destruct_one_match_hyp.
+        * apply only_differ_union_r; try apply valid_range_modVars. eapply IHfuel. eassumption.
+        * apply only_differ_union_l; try apply valid_range_modVars. eapply IHfuel. eassumption.
+      + apply invert_eval_SLoop in Ev. destruct Ev as [Ev | Ev]. 
+        * destruct Ev as [Ev C]. 
+          simpl.
+          apply only_differ_union_l; try apply valid_range_modVars. apply IHfuel. assumption.
+        * destruct Ev as [mid2 [mid3 [cv [Ev1 [C1 [C2 [Ev2 Ev3]]]]]]].
+          eapply only_differ_trans.
+          { simpl. apply only_differ_union_l; try apply valid_range_modVars.
+            apply IHfuel. eassumption. }
+          { eapply only_differ_trans.
+            { simpl. apply only_differ_union_r; try apply valid_range_modVars.
+              apply IHfuel. eassumption. }
+            { apply IHfuel. assumption. } }
+      + apply invert_eval_SSeq in Ev.
+        destruct Ev as [mid [Ev1 Ev2]]. simpl.
+        eapply only_differ_trans.
+        * apply only_differ_union_l; try apply valid_range_modVars. eapply IHfuel. eassumption.
+        * apply only_differ_union_r; try apply valid_range_modVars. eapply IHfuel. eassumption.
+      + simpl. inversionss. apply only_differ_refl.
+  Qed.
+
+  Lemma range_union_one_r: forall x1 x2 x3,
+    x1 <= x2 < x3 ->
+    range_union (x1, x3) (range_one x2) = (x1, x3).
+  Proof.
+    intros. unfold range_union, range_one.
+    repeat match goal with
+    | [ |- context[if ?e then _ else _] ] => let E := fresh "E" in destruct e eqn: E
+    end; f_equal; try omega.
+    - pose proof (Min.min_spec x1 x2). omega.
+    - pose proof (Max.max_spec x3 (S x2)). omega.
+  Qed.
+
+  Lemma range_union_inc_r: forall x1 x2,
+    x1 <= x2 ->
+    range_union (x1, x2) (range_one x2) = (x1, S x2).
+  Proof.
+    intros. unfold range_union, range_one.
+    repeat match goal with
+    | [ |- context[if ?e then _ else _] ] => let E := fresh "E" in destruct e eqn: E
+    end; f_equal; try omega.
+    - pose proof (Min.min_spec x1 x2). omega.
+    - pose proof (Max.max_spec x2 (S x2)). omega.
+  Qed.
+
+  Lemma range_union_adj: forall x1 x2 x3,
+    x1 <= x2 <= x3 ->
+    range_union (x1, x2) (x2, x3) = (x1, x3).
+  Proof.
+   unfold range_union. intros.
+    repeat match goal with
+    | [ |- context[if ?e then _ else _] ] => let E := fresh "E" in destruct e eqn: E
+    end; f_equal; try omega.
+    - pose proof (Min.min_spec x1 x2). omega.
+    - pose proof (Max.max_spec x2 x3). omega.
+  Qed.
+
+  Lemma flattenExpr_modVars_spec: forall e s firstFree resVar,
+    flattenExpr firstFree e = (s, resVar) ->
+    modVars s = (firstFree, S resVar) /\ firstFree <= resVar .
+  Proof.
+    induction e; introv E; inversions E; try (split; [reflexivity | omega]).
+    destruct (flattenExpr firstFree e1) as [p1 r1] eqn: E1.
+    destruct (flattenExpr (S r1) e2) as [p2 r2] eqn: E2.
+    inversions H0.
+    simpl.
+    specialize (IHe1 _ _ _ E1). destruct IHe1 as [IH1a IH1b].
+    specialize (IHe2 _ _ _ E2). destruct IHe2 as [IH2a IH2b].
+    rewrite IH1a, IH2a.
+    split; [|omega].
+    rewrite range_union_inc_r by omega.
+    apply range_union_adj. omega.
+  Qed.
+
+  Lemma increase_fuel_still_Success: forall fuel1 fuel2 initial s final,
+    fuel1 <= fuel2 ->
+    FlatImp.eval_stmt fuel1 initial s = Success final ->
+    FlatImp.eval_stmt fuel2 initial s = Success final.
+  Proof.
+    induction fuel1; introv L Ev.
+    - inversions Ev.
+    - destruct fuel2; [omega|]. destruct s.
+      + exact Ev.
+      + exact Ev.
+      + exact Ev.
+      + simpl in *. destruct_one_match; try discriminate.
+        erewrite IHfuel1; [reflexivity | omega | exact Ev].
+      + apply invert_eval_SLoop in Ev.
+        destruct Ev as [Ev | Ev]. 
+        * destruct Ev as [Ev C]. 
+          simpl. erewrite IHfuel1; [|omega|eassumption].
+          rewrite C. simpl. destruct_one_match; [reflexivity | contradiction].
+        * destruct Ev as [mid2 [mid3 [cv [Ev1 [C1 [C2 [Ev2 Ev3]]]]]]].
+          simpl.
+          erewrite IHfuel1; [|omega|eassumption].
+          erewrite IHfuel1; [|omega|eassumption].
+          erewrite IHfuel1; [|omega|eassumption].
+          rewrite C1. simpl.
+          destruct_one_match; [ contradiction | reflexivity ].
+     + apply invert_eval_SSeq in Ev.
+       destruct Ev as [mid [Ev1 Ev2]].
+       simpl.
+       erewrite IHfuel1; [|omega|eassumption].
+       erewrite IHfuel1; [|omega|eassumption].
+       reflexivity.
+     + simpl. inversionss. reflexivity.
+  Qed.
+
+  Lemma flattenExpr_correct_aux: forall e firstFree resVar s initialH initialL res,
+    flattenExpr firstFree e = (s, resVar) ->
+    extends initialL initialH ->
+    ExprImp.eval_expr initialH e = Some res ->
+    exists fuel finalL,
+      FlatImp.eval_stmt fuel initialL s = Success finalL /\
+      get finalL resVar = Some res /\
+      only_differ initialL (firstFree, S resVar) finalL.
+  Proof.
+    induction e; introv F Ex Ev.
+    - inversionss.
+      exists 1 (put initialL resVar res). repeat split.
+      + apply get_put_same.
+      + apply only_differ_one.
+    - inversionss.
+      exists 1 (put initialL resVar res). repeat split.
+      + simpl. unfold extends in Ex. apply Ex in H0. rewrite H0. reflexivity.
+      + rewrite get_put_same. symmetry. assumption.
+      + apply only_differ_one.
+    - inversionss. repeat (destruct_one_match_hyp; try discriminate). inversionss.
+      specialize (IHe1 _ _ _ _ _ w0 E Ex E1).
+      destruct IHe1 as [fuel1 [midL [Ev1 [G1 D1]]]].
+      specialize (IHe2 _ _ _ initialH midL w1 E0).
+      specializes IHe2.
+      { admit. (* TODO unmodified ranges... *) }
+      { assumption. }
+      destruct IHe2 as [fuel2 [preFinalL [Ev2 [G2 D2]]]].
+      remember (S (S (fuel1 + fuel2))) as f0.
+      remember (S (fuel1 + fuel2)) as f.
+      exists (S f0) (put preFinalL (S v0) (Op.eval_binop op w0 w1)).
+      repeat split.
+      + simpl. erewrite increase_fuel_still_Success; [| |eassumption]; [|omega].
+        apply increase_fuel_still_Success with (fuel1 := f0); [omega|].
+        subst f0. simpl.
+        erewrite (increase_fuel_still_Success _ _ midL); [| |eassumption]; [|omega].
+        subst f. simpl.
+        assert (get preFinalL v = Some w0) as G1' by admit. (* TODO follows from G1 and D2 *)
+        rewrite G1'. simpl. rewrite G2. simpl. reflexivity.
+      + apply get_put_same.
+      + apply only_differ_trans with (s2 := midL).
+        * admit. (* TODO follows from D1 *)
+        * eapply only_differ_trans with (s2 := preFinalL).
+          { admit. (* TODO follows from D2 *) }
+          { admit. (* TODO because changed var in range *) }
+  Qed.
+
+End FlattenExpr.
